examples/lpr_checker/array/compilation/proofs/lpr_arrayProofScript.sml
@@ -55,6 +55,100 @@ val check_unsat_code_def = Define `
   check_unsat_code = (code, data, config)
   `;
 
+Theorem lookup_build_fml:
+  ∀ls n acc i.
+  lookup i (build_fml n ls acc) =
+  if n ≤ i ∧ i < n + LENGTH ls
+  then SOME (EL (i-n) ls)
+  else lookup i acc
+Proof
+  Induct>>rw[build_fml_def]
+  >- (
+    `i-n = SUC(i-(n+1))` by DECIDE_TAC>>
+    simp[])
+  >- fs[]
+  >- (
+    `i-n=0`by fs[]>>
+    simp[lookup_insert])>>
+  simp[lookup_insert]
+QED
+
+Theorem SORTED_range:
+  SORTED  $< ls ∧
+  (∀i. MEM i ls ⇔ a ≤ i ∧ i < b) ⇒
+  ls = GENLIST ($+ a) (b-a)
+Proof
+  rw[]>>
+  match_mp_tac (SORTED_PERM_EQ |> SIMP_RULE std_ss [PULL_FORALL,AND_IMP_INTRO])>>
+  qexists_tac`$<`>>
+  CONJ_ASM1_TAC>>
+  simp[antisymmetric_def]>>
+  CONJ_ASM1_TAC>-
+    simp[SORTED_GENLIST_PLUS]>>
+  fs[]>>
+  `irreflexive ($< : num -> num -> bool)` by
+    simp[irreflexive_def]>>
+  imp_res_tac SORTED_ALL_DISTINCT>>
+  rfs[]>>
+  match_mp_tac PERM_ALL_DISTINCT>>
+  fs[MEM_GENLIST]>>
+  rw[EQ_IMP_THM]>>
+  qexists_tac`x-a`>>simp[]
+QED
+
+Theorem MAP_FST_LIST_EQ:
+  ALL_DISTINCT (MAP FST l1) ∧
+  MAP FST l1 = MAP FST l2 ∧
+  (∀x. ALOOKUP l1 (x:num) = ALOOKUP l2 x)
+  ⇒ l1 = l2
+Proof
+  rw[]>>rw[LIST_EQ_REWRITE]>-
+    metis_tac[LENGTH_MAP]>>
+  `ALOOKUP l1 (FST (EL x l1)) = SOME (SND (EL x l1))` by
+    (match_mp_tac ALOOKUP_ALL_DISTINCT_EL>>
+    fs[])>>
+  `ALOOKUP l2 (FST (EL x l2)) = SOME (SND (EL x l2))` by
+    (match_mp_tac ALOOKUP_ALL_DISTINCT_EL>>
+    fs[]>>metis_tac[LENGTH_MAP])>>
+  rfs[LIST_EQ_REWRITE,EL_MAP,LENGTH_MAP]>>
+  fs[EL_MAP]>>
+  first_x_assum drule>>
+  Cases_on`EL x l1`>> Cases_on`EL x l2`>>fs[]
+QED
+
+Theorem ALOOKUP_enumerate:
+  ∀ls k x.
+  ALOOKUP (enumerate k ls) x =
+  if k ≤ x ∧ x < LENGTH ls + k then SOME (EL (x-k) ls) else NONE
+Proof
+  Induct>>rw[miscTheory.enumerate_def]>>
+  `x-k = SUC(x-(k+1))` by DECIDE_TAC>>
+  simp[]
+QED
+
+Theorem toSortedAList_build_fml_enumerate:
+  toSortedAList (build_fml 1 ls LN) = enumerate 1 ls
+Proof
+  `MAP FST (toSortedAList (build_fml 1 ls LN)) = GENLIST ($+ 1) (LENGTH ls+1 -1)` by
+    (match_mp_tac SORTED_range>>
+    simp[SORTED_toSortedAList,MEM_MAP,EXISTS_PROD,MEM_toSortedAList]>>
+    simp[lookup_build_fml,lookup_def])>>
+  match_mp_tac MAP_FST_LIST_EQ>>
+  fs[MAP_FST_enumerate]>>
+  CONJ_ASM1_TAC
+  >-(
+    pop_assum sym_sub_tac>>
+    simp[ALL_DISTINCT_MAP_FST_toSortedAList])>>
+  rw[]>>
+  simp[ALOOKUP_toSortedAList,lookup_build_fml,ALOOKUP_enumerate,lookup_def]
+QED
+
+Theorem MAP_SND_enumerate:
+  MAP SND (enumerate k ls) = ls
+Proof
+  rw[LIST_EQ_REWRITE,LENGTH_enumerate,EL_MAP,EL_enumerate]
+QED
+
 Theorem machine_code_sound:
   wfcl cl ∧ wfFS fs ∧ STD_streams fs ∧ hasFreeFD fs ⇒
   installed_x64 check_unsat_code (basis_ffi cl fs) mc ms ⇒
@@ -64,19 +158,27 @@ Theorem machine_code_sound:
   ∃out err.
     extract_fs fs (check_unsat_io_events cl fs) =
       SOME (add_stdout (add_stderr fs err) out) ∧
-    if out = strlit "s VERIFIED UNSAT\n" then
-      (LENGTH cl = 3 ∨ LENGTH cl = 4) ∧ inFS_fname fs (EL 1 cl) ∧
-      ∃mv fml.
-        parse_dimacs (all_lines fs (EL 1 cl)) = SOME (mv,fml) ∧
-        unsatisfiable (interp fml)
+  if out = strlit "s VERIFIED UNSAT\n" then
+    LENGTH cl = 3 ∧ inFS_fname fs (EL 1 cl) ∧
+    ∃fml.
+      parse_dimacs (all_lines fs (EL 1 cl)) = SOME fml ∧
+      unsatisfiable (interp fml)
+  else if out = strlit "s VERIFIED TRANSFORMATION\n" then
+    LENGTH cl = 4 ∧ inFS_fname fs (EL 1 cl) ∧ inFS_fname fs (EL 3 cl) ∧
+    ∃fml fml2.
+      parse_dimacs (all_lines fs (EL 1 cl)) = SOME fml ∧
+      parse_dimacs (all_lines fs (EL 3 cl)) = SOME fml2 ∧
+      (satisfiable (interp fml) ⇒ satisfiable (interp fml2))
+  else if LENGTH cl = 2 then
+    if inFS_fname fs (EL 1 cl)
+    then
+      case parse_dimacs (all_lines fs (EL 1 cl)) of
+        NONE => out = strlit ""
+      | SOME fml => out = concat (print_dimacs fml)
     else
-      if LENGTH cl = 2 ∧ inFS_fname fs (EL 1 cl)
-      then
-        case parse_dimacs (all_lines fs (EL 1 cl)) of
-          NONE => out = strlit ""
-        | SOME (mv,fml) => out = concat (print_dimacs fml)
-      else
-        out = strlit ""
+      out = strlit ""
+  else
+    out = strlit ""
 Proof
   ntac 2 strip_tac>>
   fs[installed_x64_def,check_unsat_code_def]>>
@@ -86,115 +188,159 @@ Proof
   disch_then (qspecl_then [`ms`,`mc`,`data_sp`,`cbspace`] mp_tac)>>
   simp[]>> strip_tac>>
   fs[check_unsat_sem_def]>>
-  TOP_CASE_TAC>- (
-    fs[]>>
-    qexists_tac`strlit ""`>>simp[]>>
-    qexists_tac`err`>>rw[]
-    >-
-      metis_tac[STD_streams_add_stderr, STD_streams_stdout,add_stdo_nil]>>
-    fs[parse_arguments_def]>>
-    every_case_tac>>fs[]>>
-    Cases_on`cl`>>fs[])>>
-  TOP_CASE_TAC >>fs[]>>
-  reverse IF_CASES_TAC>>fs[] >- (
-    qexists_tac`strlit ""`>>simp[]>>
-    qexists_tac`err`>>rw[]
-    >-
-      metis_tac[STD_streams_add_stderr, STD_streams_stdout,add_stdo_nil]>>
-    fs[parse_arguments_def]>>
-    every_case_tac>>fs[]>>
-    Cases_on`cl`>>fs[])>>
-  TOP_CASE_TAC>>fs[]
-  >-
-     metis_tac[STD_streams_add_stderr, STD_streams_stdout,add_stdo_nil]>>
-  TOP_CASE_TAC>>fs[]>>
-  TOP_CASE_TAC>>fs[]
+  Cases_on`cl`>>fs[]
   >- (
-    (* print DIMACS case *)
-    qexists_tac`concat (print_dimacs r')`>>
+    (* 0 arg *)
+    fs[]>>
+    qexists_tac`err`>>rw[]>>
+    metis_tac[STD_streams_add_stderr, STD_streams_stdout,add_stdo_nil])>>
+  TOP_CASE_TAC >> fs[] >- (
+    qexists_tac`err`>>rw[]>>
+    metis_tac[STD_streams_add_stderr, STD_streams_stdout,add_stdo_nil])>>
+  TOP_CASE_TAC
+  >-(
+    (* 1 arg *)
+    fs[check_unsat_1_sem_def]>>
+    reverse IF_CASES_TAC>>fs[]
+    >- (
+      qexists_tac`err`>>rw[]
+      >- metis_tac[STD_streams_add_stderr, STD_streams_stdout,add_stdo_nil]>>
+      Cases_on`cl`>>rfs[])>>
+    TOP_CASE_TAC>>fs[]
+    >- (
+      qexists_tac`strlit ""`>>simp[]>>
+      qexists_tac`err`>>rw[]
+      >- metis_tac[STD_streams_add_stderr, STD_streams_stdout,add_stdo_nil]>>
+      fs[parse_dimacs_def])>>
+    PairCases_on`x`>>fs[]>>
+    qexists_tac`concat (print_dimacs_toks x2)`>>
     qexists_tac`strlit ""` >>
     simp[STD_streams_stderr,add_stdo_nil]>>
-    simp[print_dimacs_def]>>
-    `?x. cl = [x;q]` by
-      (fs[parse_arguments_def]>>every_case_tac>>fs[]>>
-      Cases_on`cl`>>fs[])>>
-    fs[]>>
+    simp[parse_dimacs_def,print_dimacs_def,toSortedAList_build_fml_enumerate,MAP_SND_enumerate]>>
+    simp[print_dimacs_toks_def]>>
     simp[print_header_line_def]>>
     qmatch_goalsub_abbrev_tac` (strlit"p cnf " ^ a ^ b ^ c)`>>
     qmatch_goalsub_abbrev_tac` _ :: d`>>
     EVAL_TAC)>>
-  TOP_CASE_TAC>>fs[]>>
-  reverse TOP_CASE_TAC>>fs[]
-  >- (
-    qexists_tac`strlit ""`>>simp[]>>
-    qexists_tac`err`>>rw[]
-    >-
-      metis_tac[STD_streams_add_stderr, STD_streams_stdout,add_stdo_nil]>>
-    fs[parse_arguments_def]>>
-    every_case_tac>>fs[]>>
-    Cases_on`cl`>>fs[])>>
   TOP_CASE_TAC>>fs[]
   >- (
-    qexists_tac`strlit ""`>>simp[]>>
-    qexists_tac`err`>>rw[]
-    >-
-      metis_tac[STD_streams_add_stderr, STD_streams_stdout,add_stdo_nil]>>
-    fs[parse_arguments_def]>>
-    every_case_tac>>fs[]>>
-    Cases_on`cl`>>fs[])>>
-  reverse IF_CASES_TAC >> fs[] >- (
-    qexists_tac`strlit ""`>>simp[]>>
-    qexists_tac`err`>>rw[]
-    >-
-      metis_tac[STD_streams_add_stderr, STD_streams_stdout,add_stdo_nil]>>
-    fs[parse_arguments_def]>>
-    every_case_tac>>fs[]>>
-    Cases_on`cl`>>fs[])>>
-  (* the actual interesting case *)
-  qexists_tac`strlit "s VERIFIED UNSAT\n"` >> qexists_tac`strlit ""`>> simp[]>>
-  CONJ_TAC >-
-    metis_tac[STD_streams_stderr,add_stdo_nil]>>
-  PURE_REWRITE_TAC[CONJ_ASSOC]>>
-  CONJ_TAC>-
-    (fs[parse_arguments_def]>>every_case_tac>>fs[]>>
-    Cases_on`cl`>>fs[])>>
-  drule (check_lpr_unsat_list_sound)>>simp[]>>
-  disch_then match_mp_tac>>
-  metis_tac[parse_dimacs_wf_bound,parse_lpr_wf]
-QED
-
-Theorem machine_code_sound_parse_print:
-  wfcl cl ∧ wfFS fs ∧ STD_streams fs ∧ hasFreeFD fs ⇒
-  installed_x64 check_unsat_code (basis_ffi cl fs) mc ms ⇒
-  machine_sem mc (basis_ffi cl fs) ms ⊆
-    extend_with_resource_limit
-      {Terminate Success (check_unsat_io_events cl fs)} ∧
-  (* If we start with a well-formed formula, and put it into the file *)
-  wf_fml fml ∧ inFS_fname fs (EL 1 cl) ∧ all_lines fs (EL 1 cl) = print_dimacs fml ⇒
-  ∃out err.
-    extract_fs fs (check_unsat_io_events cl fs) = SOME (add_stdout (add_stderr fs err) out) ∧
-    (* Then if the output is "s VERIFIED UNSAT\n" that formula was also unsatisfiable *)
-    if out = strlit "s VERIFIED UNSAT\n" then
-      (LENGTH cl = 3 ∨ LENGTH cl = 4) ∧ unsatisfiable (interp fml)
-    else
-      if LENGTH cl = 2 then
-        ∃fml'.
-        interp fml = interp fml' ∧ out = concat (print_dimacs fml')
-      else out = strlit ""
-Proof
-  rw[]>>
-  drule machine_code_sound>>
-  rpt(disch_then drule>>simp[])>>
-  strip_tac>>
-  asm_exists_tac>> simp[] >>
-  IF_CASES_TAC
+    (* 2 arg *)
+    fs[check_unsat_2_sem_def]>>
+    reverse IF_CASES_TAC>>fs[]
+    >- (
+      qexists_tac`err`>>rw[]
+      >- metis_tac[STD_streams_add_stderr, STD_streams_stdout,add_stdo_nil]>>
+      Cases_on`cl`>>rfs[])>>
+    TOP_CASE_TAC>>fs[]
+    >- (
+      qexists_tac`strlit ""`>>simp[]>>
+      qexists_tac`err`>>rw[]
+      >- metis_tac[STD_streams_add_stderr, STD_streams_stdout,add_stdo_nil]>>
+      fs[parse_dimacs_def])>>
+    PairCases_on`x`>>fs[]>>
+    reverse IF_CASES_TAC>>fs[]
+    >- (
+      qexists_tac`strlit ""`>>simp[]>>
+      qexists_tac`err`>>rw[]
+      >- metis_tac[STD_streams_add_stderr, STD_streams_stdout,add_stdo_nil]>>
+      fs[parse_dimacs_def]) >>
+    TOP_CASE_TAC>>fs[]
+    >- (
+      qexists_tac`strlit ""`>>simp[]>>
+      qexists_tac`err`>>rw[]
+      >- metis_tac[STD_streams_add_stderr, STD_streams_stdout,add_stdo_nil]>>
+      fs[parse_dimacs_def]) >>
+    reverse IF_CASES_TAC>>fs[]
+    >- (
+      qexists_tac`strlit ""`>>simp[]>>
+      qexists_tac`err`>>rw[]
+      >- metis_tac[STD_streams_add_stderr, STD_streams_stdout,add_stdo_nil]>>
+      fs[parse_dimacs_def]) >>
+    qexists_tac`strlit "s VERIFIED UNSAT\n"` >>
+    qexists_tac`strlit ""`>> simp[]>>
+    CONJ_TAC >-
+      metis_tac[STD_streams_stderr,add_stdo_nil]>>
+    fs[parse_dimacs_def]>>
+    fs[GSYM toSortedAList_build_fml_enumerate]>>
+    drule (check_lpr_unsat_list_sound)>>simp[]>>
+    disch_then match_mp_tac>>
+    CONJ_TAC >- (
+      match_mp_tac (GEN_ALL parse_dimacs_wf)>>simp[parse_dimacs_def]>>
+      qexists_tac`all_lines fs h'`>>fs[])>>
+    metis_tac[parse_lpr_wf])>>
+  reverse TOP_CASE_TAC>>fs[]
   >- (
-    drule parse_dimacs_print_dimacs>> rw[]>>
-    fs[interp_def]>>
-    rw[]) >>
-  fs[]>> rw[] >> fs[]>>
-  drule parse_dimacs_print_dimacs>> rw[]>> fs[]>>
-  qexists_tac`fml'`>> simp[interp_def]
+    qexists_tac`err`>>rw[]
+    >- metis_tac[STD_streams_add_stderr, STD_streams_stdout,add_stdo_nil]>>
+    Cases_on`cl`>>rfs[])
+  >>
+    (* 3 arg *)
+    fs[check_unsat_3_sem_def]>>
+    reverse IF_CASES_TAC>>fs[]
+    >- (
+      qexists_tac`err`>>rw[]
+      >- metis_tac[STD_streams_add_stderr, STD_streams_stdout,add_stdo_nil]>>
+      Cases_on`cl`>>rfs[])>>
+    TOP_CASE_TAC>>fs[]
+    >- (
+      qexists_tac`strlit ""`>>simp[]>>
+      qexists_tac`err`>>rw[]
+      >- metis_tac[STD_streams_add_stderr, STD_streams_stdout,add_stdo_nil]>>
+      fs[parse_dimacs_def])>>
+    PairCases_on`x`>>fs[]>>
+    reverse IF_CASES_TAC>>fs[]
+    >- (
+      qexists_tac`err`>>rw[]
+      >- metis_tac[STD_streams_add_stderr, STD_streams_stdout,add_stdo_nil]>>
+      fs[parse_dimacs_def]) >>
+    TOP_CASE_TAC>>fs[]
+    >- (
+      qexists_tac`strlit ""`>>simp[]>>
+      qexists_tac`err`>>rw[]
+      >- metis_tac[STD_streams_add_stderr, STD_streams_stdout,add_stdo_nil]>>
+      fs[parse_dimacs_def]) >>
+    PairCases_on`x`>>fs[]>>
+    reverse IF_CASES_TAC>>fs[]
+    >- (
+      qexists_tac`strlit ""`>>simp[]>>
+      qexists_tac`err`>>rw[]
+      >- metis_tac[STD_streams_add_stderr, STD_streams_stdout,add_stdo_nil]>>
+      fs[parse_dimacs_def]) >>
+    TOP_CASE_TAC>>fs[]
+    >- (
+      qexists_tac`strlit ""`>>simp[]>>
+      qexists_tac`err`>>rw[]
+      >- metis_tac[STD_streams_add_stderr, STD_streams_stdout,add_stdo_nil]>>
+      fs[parse_dimacs_def]) >>
+    reverse IF_CASES_TAC>>fs[]
+    >- (
+      qexists_tac`strlit ""`>>simp[]>>
+      qexists_tac`err`>>rw[]
+      >- metis_tac[STD_streams_add_stderr, STD_streams_stdout,add_stdo_nil]>>
+      fs[parse_dimacs_def]) >>
+    qexists_tac`strlit "s VERIFIED TRANSFORMATION\n"` >>
+    qexists_tac`strlit ""`>> simp[]>>
+    CONJ_TAC >-
+      metis_tac[STD_streams_stderr,add_stdo_nil]>>
+    fs[parse_dimacs_def]>>
+    fs[GSYM toSortedAList_build_fml_enumerate]>>
+    drule (check_lpr_sat_equiv_list_sound)>>simp[]>>
+    `IMAGE interp_cclause (set x2') =
+      interp (build_fml 1 x2' LN)` by
+      (simp[interp_def,values_def,lookup_build_fml]>>
+      AP_TERM_TAC>>
+      rw[EXTENSION,lookup_def]>>
+      simp[MEM_EL]>>
+      rw[EQ_IMP_THM]
+      >- (qexists_tac`n+1`>>simp[])>>
+      qexists_tac`n-1`>>simp[])>>
+    simp[]>>
+    rw[]>>fs[]>>
+    first_x_assum match_mp_tac>>
+    CONJ_TAC >- (
+      match_mp_tac (GEN_ALL parse_dimacs_wf)>>simp[parse_dimacs_def]>>
+      qexists_tac`all_lines fs h'`>>fs[])>>
+    metis_tac[parse_lpr_wf]
 QED
 
 val _ = export_theory();
